testcases/printtest/test_with_function.c
@@ -141,8 +141,8 @@ int main() {
 //    test_1();
 // Passed
 //    test_2();
-    test_3();
-//    test_4();
+//    test_3();
+    test_4();
 //    test_5();
 //    test_6();
     return 0;
